Add inductive phi proofs

Star/ARS.lean
@@ -6,21 +6,30 @@ Released under Apache 2.0 license as described in the file LICENSE.
 namespace Star
 
 @[simp] abbrev Rule (A : Type _) := A → A → Prop
+@[simp] abbrev Method (A : Type _) (E : Type _) := A → E → A → Prop -- B is the equeu element
 
 structure ARS (I : Type _) where
   A : Type _
   rules : I → Rule A
 
 inductive trans {A} (rule : Rule A) : Rule A where
-| step {a b c} : rule a b → trans rule b c → trans rule a c
+| step {a b c} : trans rule a b → rule b c→ trans rule a c
 | refl {a b} : rule a b → trans rule a b
 
 def refl {A} (rule : Rule A) (s e : A) : Prop :=
   rule s e ∨ s = e
 
+
+-- this is the star and then the user give me A as a union of all possibile rule R1, R2, R3 ecc...
 inductive trans_refl {A} (rule : Rule A) : Rule A where
-| step {a b c} : trans_refl rule a b → rule b c → trans_refl rule a c
+| step {a b c} : rule a b → trans_refl rule b c → trans_refl rule a c
 | refl {a} : trans_refl rule a a
+
+inductive trans_refl2 {A} (rule : Rule A) : Rule A where
+| step {a b c} : rule b c → trans_refl2 rule a b → trans_refl2 rule a c
+| refl {a} : trans_refl2 rule a a
+
+
 
 inductive counted_trans_refl {A} (rule : Rule A) : A → A → Nat → Prop where
 | step {a b c n} : rule a b → counted_trans_refl rule b c n → counted_trans_refl rule a c (n+1)
@@ -36,6 +45,8 @@ def union {A} (α β : Rule A) (s e : A) : Prop := α s e ∨ β s e
 def inv {A} (α : Rule A) (s e : A) : Prop := α e s
 def symm {A} (α : Rule A) : Rule A := union α (inv α)
 def compose {A} (α β : Rule A) (s e : A) : Prop := ∃ s', α s s' ∧ β s' e
+
+
 
 def commutes_weakly {A} (α β : Rule A) :=
   ∀ {a b c : A}, β a c → α a b → ∃ d, trans_refl α c d ∧ trans_refl β b d
@@ -65,6 +76,14 @@ inductive strongly_normalising' {A} (α : Rule A) : A → Prop where
 
 def strongly_normalising {A} (α : Rule A) := ∀ a, strongly_normalising' α a
 
+#print Acc
+
+inductive well_founded' {A} (α : Rule A) : A → Prop where
+| step {b} : (∀ a, α a b → well_founded' α a) → well_founded' α b
+
+def well_founded {A} (α : Rule A) := ∀ a, well_founded' α a
+
+
 def is_inductive {A} (α : Rule A) :=
   ∀ a b n, counted_trans_refl α a b n → ∃ a', trans_refl α b a'
 
@@ -85,6 +104,10 @@ example : ARS.indexed_red_seq ars [true, false, true] true true := by repeat con
 
 end Example
 
+/-
+# Newmans proofs
+-/
+
 @[simp]
 theorem double_application_term {A} (α: Rule A) :
   ∀ {a b: A},  α a b -> trans_refl α a b := by
@@ -93,6 +116,12 @@ theorem double_application_term {A} (α: Rule A) :
   exact h
   apply trans_refl.refl
 
+
+
+
+@[simp]
+theorem double_application_term' {A} (α: Rule A) :
+  ∀ {a b: A},  α a b -> trans α a b := by grind[trans.refl]
 
 
 @[simp]
@@ -106,37 +135,232 @@ theorem double_application_term1 {A} (α: Rule A) :
   case refl a =>
     apply trans_refl.refl
 
+@[simp]
+theorem double_application_term2 {A} (α: Rule A) :
+  ∀ {a b: A},  trans_refl (trans_refl α) a b  -> trans_refl α a b := by
+  intro a b h
+  induction h
+  . clear a b
+    rename_i a b c h1 h2 h3
+    clear h2
+    induction h1
+    . clear a b
+      rename_i a b d e h1 h2
+      specialize h2 h3
+      constructor <;> assumption
+    . assumption
+  . apply trans_refl.refl
 
 
-theorem confleunt {A} (α : Rule A) : has_diamond_property α → is_confluent α := by
+
+
+-- theorem confleunt {A} (α : Rule A) : has_diamond_property α → is_confluent α := by
+--   intro h
+--   unfold is_confluent commutes commutes_weakly
+--   intro a b c t1 t2
+--   unfold has_diamond_property at h
+--   revert t2 b
+--   induction t1
+--   . rename_i a' b' c' h1 h2 ih
+--     intro b t2
+--     clear a c
+--     cases h' : t2
+--     . rename_i z h4 h5
+--       specialize h h1 h4
+--       cases h; rename_i d' h
+--       rcases h with ⟨H1, H2⟩
+--       have H1' := trans_refl.step H1 trans_refl.refl
+--       specialize ih H1'
+--       cases ih; rename_i d'' h'
+--       rcases h' with ⟨H3, H4⟩
+--       have H2' : trans_refl α z d'' := by admit
+--       clear H4 H3 H1' H2 H1 h2 h1 h' h4
+--       induction t2
+--       . rename_i z' b'' c'' h3 h4 ih'
+--         specialize ih' h5
+--         assumption
+--       . admit
+--     . admit
+--   . admit
+
+
+theorem termination {A} (α : Rule A) : strongly_normalising α → well_founded (inv α) := by
+  intro h a
+  specialize h a
+  induction h
+  case step a h1 ih =>
+    apply well_founded'.step
+    intro b h2
+    specialize ih b h2
+    assumption
+
+
+
+
+theorem termination_steps' {A} (α : Rule A) : well_founded α -> well_founded (trans α) := by
+  intro h a
+  apply well_founded'.step
+  specialize h a
+  intro b h2
+  induction h generalizing b
+  . rename_i xa xb xc
+    cases h2
+    . grind
+    . constructor
+      grind
+
+
+theorem Newmans_lemma {A} (α : Rule A) :
+  strongly_normalising α →  has_diamond_property α → is_confluent α := by
   intro h
+  have h1 := termination α h
+  have h2 := termination_steps' (inv α) h1
+  clear h1
+  intro h1
+  unfold well_founded at h2
   unfold is_confluent commutes commutes_weakly
-  intro a b c t1 t2
-  unfold has_diamond_property at h
-  --have t1' := @double_application_term A α a b
-  --have t1 := trans_refl.refl α a
-  revert t2 b
-  induction t1
-  . rename_i a' b' c' h1 h2 ih
-    intro b t2
-    clear a c
-    generalize a' = a at *
-    generalize c' = c at *
-    clear a' c'
-    induction t2 generalizing b' c
-    . rename_i a b'' b h3 h4 ih2
+  intro a --b c t1 t2
+  specialize h2 a
+  induction h2
+  rename_i a h3 ih; rename_i a'; clear a'
+  apply ih
+  apply trans.refl
+  unfold inv
+  unfold has_diamond_property at h1
+  specialize @h1 a a a
+  admit
 
-      have H4 := h4 h1 h2 ih
-      have H4' := h4 d'' h3
-      specialize ih d''
-      specialize h a'
-    . admit
-  case refl a' =>
-    exists b
-    constructor
-    . apply double_application_term1
-      exact t2
-    . apply trans_refl.refl
+/-
+# Newmans  thorems implies refinment
+-/
+
+
+/-
+# Define i and s and φ
+-/
+
+
+
+--how the state of the implemenattion and spec are related when they are both in a flush state v
+variable {A B E}
+variable (flush : A -> B -> Prop)
+variable (rule : Rule A)
+variable (method_i : Method A E)
+variable (method_s : Method B E)
+
+
+def indistinguishability (i : A) (s : B) : Prop := ∀ (i' : A) e, method_i i e i' -> ∃ s', method_s s e s'
+
+
+inductive φ : A -> B -> Prop where
+| base : ∀ (i : A) (s : B),
+          flush i s ->
+          φ i s
+| rule_step : ∀ (i i' : A) (s : B),
+              φ i' s ->
+              trans_refl rule i i' ->
+              φ i s
+-- | method_step : ∀ (i i' : A) (s s' : B) (method_i : Method A) (method_s : Method B) n, --maybe add the forall trick
+--               φ i' s' ->
+--               method_i i n i' ->
+--               method_s s n s' ->
+--               φ i s
+
+
+theorem relation_flush : ∀ (i i' : A) (s : B) (rule : Rule A), flush i s -> trans_refl rule i i' -> flush i' s := by admit
+theorem relation_flush_method : ∀ (i i' : A) (s s' : B) e, flush i s -> method_i i e i' -> method_s s e s' ->
+                                ∃ i'', trans_refl rule i' i'' ∧ flush i'' s'  := by admit
+theorem relation_method : ∀ (i i' : A) (s : B) e, flush i s -> method_i i e i' -> ∃ s', method_s s e s' := by admit
+
+
+theorem enoght_internal (i : A) (s : B) :
+    φ flush rule i s -> ∀ i', trans_refl rule i i' -> strongly_normalising (trans_refl rule) -> has_diamond_property (trans_refl rule) -> φ flush rule i' s := by
+      intro hφ i' hstep hs hconf
+      induction hφ generalizing i'
+      . rename_i i s' h3
+        constructor
+        apply relation_flush <;> assumption
+      . clear i s
+        rename_i i i'' s h1 h2 h4
+        have H := @Newmans_lemma A (trans_refl rule) hs hconf
+        unfold is_confluent at H
+        unfold commutes at H
+        unfold commutes_weakly at H
+        have h2' := double_application_term1 _ h2
+        have hstep' := double_application_term1 _ hstep
+        specialize @H i i'' i' hstep' h2'
+        cases H; rename_i d H; rcases H with ⟨H1, H2⟩
+        have H2' := double_application_term2 _ (double_application_term2 _ H2)
+        have H1' := double_application_term2 _ (double_application_term2 _ H1)
+        specialize h4 d H2'
+        apply φ.rule_step _ d _ <;> try assumption
+
+
+def commutes_weakly_methods_i (α : Method A E) :=
+  ∀ {a b c : A} { e e' : E}, α a e c → α a e' b → ∃ d, α c e' d ∧  α b e d
+
+def commutes_weakly_methods_s (α : Method B E) :=
+  ∀ {a b c : B} { e e' : E}, α a e c → α a e' b → ∃ d, α c e' d ∧  α b e d
+
+def commutes_weakly_method_rule (α : Method A E) ( β : Rule A) :=
+  ∀ {a b c : A} { e : E}, trans_refl β a b → α a e c → ∃ d, α b e d ∧ trans_refl β c d
+
+
+theorem indistinguisability_preservation (i : A) (s : B) :
+    φ flush rule i s -> commutes_weakly_method_rule method_i rule -> @indistinguishability  _ _ E method_i method_s i s := by
+      intro h1 h2
+      induction h1
+      . clear i s
+        rename_i i s h3
+        unfold indistinguishability
+        intro i' e h4
+        apply relation_method <;> assumption
+      . clear i s
+        rename_i i i' s h3 h4 h5
+        unfold indistinguishability at *
+        intro i'' e h6
+        unfold commutes_weakly_method_rule at *
+        specialize h2 h4 h6
+        cases h2; rename_i d h2; cases h2; rename_i h2 h2'
+        apply h5 <;> assumption
+
+
+
+theorem enoght_external (i : A) (s : B) :
+    φ flush rule i s ->
+    commutes_weakly_method_rule method_i rule ->
+    ∀ i' e, method_i i e i' ->
+    ∃ (s' : B), method_s s e s' ∧ φ flush rule i' s' := by
+      intro hφ h1 i' e h4
+      have hi := @indistinguisability_preservation _ _ E _ _ method_i method_s _ _ hφ h1
+      induction hφ generalizing i'
+      . clear i s
+        rename_i i s h5
+        unfold indistinguishability at *
+        specialize hi i' e h4
+        cases hi; rename_i s' hi
+        constructor; rotate_left
+        . exact s'
+        . constructor
+          . assumption
+          . have H := @relation_flush_method A B E flush rule method_i method_s i i' s s' e h5 h4 hi
+            cases H; rename_i i'' H; cases H; rename_i H1 H2
+            apply φ.rule_step _ i''
+            . constructor; assumption
+            . assumption
+      . clear i s
+        rename_i i i'' s h5 h6 h7
+        unfold commutes_weakly_method_rule at *
+        specialize @h1 i i'' i' e h6 h4
+        cases h1; rename_i d h1; cases h1; rename_i h1 h1'
+        have H' := @indistinguisability_preservation _ _ E _ _ method_i method_s _ _ h5
+        specialize h7 d h1 (by sorry)
+        cases h7; rename_i s' h7; rcases h7 with ⟨ h7, h7'⟩
+        constructor; rotate_left; exact s'
+        constructor
+        . assumption
+        . apply φ.rule_step _ d _ <;> try assumption
+
 
 
 
