lakefile.lean
@@ -1,0 +1,8 @@
+import Lake
+open Lake DSL
+
+package «paxos» where
+  -- add package configuration options here
+
+require mathlib from git
+  "https://github.com/leanprover-community/mathlib4"
